refactor: rename SEnv.regs to SEnv.locals (#112)

EffectSSA/ProofSketch/ProofSketch.lean
@@ -38,8 +38,8 @@ A stateful environment `e : SEnv`
 bundles a pure environment with a global state.
 -/
 structure SEnv where
-  /-- A partial map from variables (i.e, virtual registers) to values. -/
-  regs : VarId → Option Val := fun _ => none
+  /-- A partial map from local variables (i.e, virtual registers) to values. -/
+  locals : VarId → Option Val := fun _ => none
   /-- The global state, e.g, for memory and UB -/
   state : State := .initial
 
@@ -95,11 +95,11 @@ theorem Pattern.denote_cons  (is : InstSeq) (I : Pattern n) :
 variable {x : VarId}
 
 /-- Instructions only modify the registers in their `results` set. -/
-@[grind .] axiom Inst.regs_denote_of_not_mem_results (i : Inst) {x : VarId} {ρ : SEnv}
-    (h : x ∉ i.results) : (⟦i⟧ ρ).regs x = ρ.regs x
+@[grind .] axiom Inst.locals_denote_of_not_mem_results (i : Inst) {x : VarId} {ρ : SEnv}
+    (h : x ∉ i.results) : (⟦i⟧ ρ).locals x = ρ.locals x
 
-@[grind =] theorem InstSeq.regs_denote_of_not_mem_results (h : x ∉ is.results) :
-    (⟦is⟧ ρ).regs x = ρ.regs x := by
+@[grind =] theorem InstSeq.locals_denote_of_not_mem_results (h : x ∉ is.results) :
+    (⟦is⟧ ρ).locals x = ρ.locals x := by
   induction is generalizing ρ <;> grind
 
 end Properties
@@ -158,15 +158,15 @@ types is all that we need to compare.
 -/
 def SEnv.EquivOn (P : VarId → Prop) : SEnv → SEnv → Prop := fun ρ η =>
   ρ.state = η.state
-  ∧ (∀ v, P v → ρ.regs v = η.regs v)
+  ∧ (∀ v, P v → ρ.locals v = η.locals v)
 
 /-- If two environments are equivalent on all variables, they are equal. -/
 theorem SEnv.eq_of_equivOn {ρ η} : EquivOn (fun _ => True) ρ η → ρ = η := by
-  rcases ρ with ⟨ρ_regs, ρ_state⟩
-  rcases η with ⟨η_regs, η_state⟩
+  rcases ρ with ⟨ρ_locals, ρ_state⟩
+  rcases η with ⟨η_locals, η_state⟩
   simp only [EquivOn]
   intro h
-  have : ρ_regs = η_regs := by funext; simp_all
+  have : ρ_locals = η_locals := by funext; simp_all
   simp_all
 
 section Lemmas
@@ -206,7 +206,7 @@ We say that `ρ` is a sub-environment of `η`, written as `ρ ⊒ η`,
     the value `ρ v` is refined by `η v`.
 -/
 instance : Refinement SEnv where
-  IsRefinedBy ρ η := ρ.state ⊒ η.state ∧ (∀ v, ρ.regs v ⊒ η.regs v)
+  IsRefinedBy ρ η := ρ.state ⊒ η.state ∧ (∀ v, ρ.locals v ⊒ η.locals v)
   antisymm := by
     rintro ⟨s, ρ⟩ ⟨t, η⟩ hxy hyx
     suffices s = t ∧ ρ = η by grind
@@ -245,7 +245,7 @@ end Refine
 section EqnLemma
 
 def Inst.EqnLemma (i : Inst) (x : VarId) (ρ : SEnv) : Prop :=
-  x ∈ i.results → (⟦i⟧ ρ).regs x = ρ.regs x
+  x ∈ i.results → (⟦i⟧ ρ).locals x = ρ.locals x
 
 @[grind] def InstSeq.EqnLemma (is : InstSeq) (x : VarId) (ρ : SEnv) : Prop :=
   ∀ i ∈ is, i.EqnLemma x ρ
@@ -366,13 +366,13 @@ theorem Inst.eqnLemma_of_eqnLemma_instSeq {i : Inst} (hi : i.HasEqn) :
 
 /-! denote lemmas -/
 
-@[grind =] theorem Inst.regs_denote_of_eqnLemma {i : Inst}
-    (h : i.EqnLemma x ρ) : (⟦i⟧ ρ).regs x = ρ.regs x := by
+@[grind =] theorem Inst.locals_denote_of_eqnLemma {i : Inst}
+    (h : i.EqnLemma x ρ) : (⟦i⟧ ρ).locals x = ρ.locals x := by
   grind [EqnLemma]
 
-@[grind .] theorem InstSeq.regs_denote_of_eqnLemma {is : InstSeq} (hEqn : is.HasEqn)
+@[grind .] theorem InstSeq.locals_denote_of_eqnLemma {is : InstSeq} (hEqn : is.HasEqn)
     (hwf : is.NoShadowing) (h : is.EqnLemma x ρ) :
-    (⟦is⟧ ρ).regs x = ρ.regs x := by
+    (⟦is⟧ ρ).locals x = ρ.locals x := by
   induction is generalizing ρ
   · rfl
   · grind
